AbstractPlatform/IntegrityProof.bpl
@@ -513,11 +513,9 @@ procedure ProveIntegrity()
         invariant (forall e : tap_enclave_id_t :: 
                 (tap_enclave_metadata_valid_1[e] && tap_enclave_metadata_privileged_1[e]) ==> 
                     distant_parent(tap_enclave_metadata_owner_map_1, e, kmax_depth_t) == tap_null_enc_id);
-                    // pe_farthest_parent(tap_enclave_metadata_owner_map_1, e) == tap_null_enc_id);
         invariant (forall e : tap_enclave_id_t :: 
                 (tap_enclave_metadata_valid_2[e] && tap_enclave_metadata_privileged_2[e]) ==> 
                     distant_parent(tap_enclave_metadata_owner_map_2, e, kmax_depth_t) == tap_null_enc_id);
-                    // pe_farthest_parent(tap_enclave_metadata_owner_map_2, e) == tap_null_enc_id);
 
         // valid guarantee
         invariant tap_enclave_metadata_valid_1[tap_null_enc_id];
@@ -544,19 +542,39 @@ procedure ProveIntegrity()
             distant_parent(tap_enclave_metadata_owner_map_1, e, kmax_depth_t+1) == tap_null_enc_id);
         invariant (forall e : tap_enclave_id_t :: tap_enclave_metadata_valid_2[e] ==> 
             distant_parent(tap_enclave_metadata_owner_map_2, e, kmax_depth_t+1) == tap_null_enc_id);
-            // farthest_parent(tap_enclave_metadata_owner_map_1, eid) == tap_null_enc_id);
-            // farthest_parent(tap_enclave_metadata_owner_map_2, eid) == tap_null_enc_id);
+        
+        // invariants about 'distant_parent'
+        // We give constructive evidences of 'distant_parent'
+        invariant (forall n : int :: 
+            distant_parent(tap_enclave_metadata_owner_map_1, tap_null_enc_id, n) == tap_null_enc_id);
+        invariant (forall n : int ::
+            distant_parent(tap_enclave_metadata_owner_map_2, tap_null_enc_id, n) == tap_null_enc_id);
+        
+        invariant (forall e : tap_enclave_id_t :: tap_enclave_metadata_valid_1[e] ==> 
+            distant_parent(tap_enclave_metadata_owner_map_1, e, 1) == tap_enclave_metadata_owner_map_1[e]);
+        invariant (forall e : tap_enclave_id_t :: tap_enclave_metadata_valid_2[e] ==> 
+            distant_parent(tap_enclave_metadata_owner_map_2, e, 1) == tap_enclave_metadata_owner_map_2[e]);
+        
+        invariant (forall e : tap_enclave_id_t :: tap_enclave_metadata_valid_1[e] ==> 
+            (forall n1, n2 : int :: (is_valid_depth(n1) && is_valid_depth(n2) && (is_valid_depth(n1 + n2))) ==> 
+                distant_parent(tap_enclave_metadata_owner_map_1, distant_parent(tap_enclave_metadata_owner_map_1, e, n1), n2) == 
+                distant_parent(tap_enclave_metadata_owner_map_1, e, n1 + n2)));
+        invariant (forall e : tap_enclave_id_t :: tap_enclave_metadata_valid_2[e] ==> 
+            (forall n1, n2 : int :: (is_valid_depth(n1) && is_valid_depth(n2) && (is_valid_depth(n1 + n2))) ==> 
+                distant_parent(tap_enclave_metadata_owner_map_2, distant_parent(tap_enclave_metadata_owner_map_2, e, n1), n2) == 
+                distant_parent(tap_enclave_metadata_owner_map_2, e, n1 + n2)));
 
-        // invariant (forall e : tap_enclave_id_t :: (tap_enclave_metadata_valid_1[e]) ==> 
-        //             (tap_enclave_metadata_owner_map_1[tap_enclave_metadata_owner_map_1[e]] == tap_null_enc_id));
-        // invariant (forall e : tap_enclave_id_t :: (tap_enclave_metadata_valid_2[e]) ==> 
-        //             (tap_enclave_metadata_owner_map_2[tap_enclave_metadata_owner_map_2[e]] == tap_null_enc_id));
+        invariant (forall e : tap_enclave_id_t :: tap_enclave_metadata_valid_1[e] ==> 
+            (exists n : int :: (is_valid_depth(n) && (n < kmax_depth_t+1) && distant_parent(tap_enclave_metadata_owner_map_1, e, n) == tap_null_enc_id) ==> 
+                (forall m : int :: (m > n && m < kmax_depth_t+1) ==> 
+                    distant_parent(tap_enclave_metadata_owner_map_1, e, m) == tap_null_enc_id)));
+        invariant (forall e : tap_enclave_id_t :: tap_enclave_metadata_valid_2[e] ==> 
+            (exists n : int :: (is_valid_depth(n) && (n < kmax_depth_t+1) && distant_parent(tap_enclave_metadata_owner_map_2, e, n) == tap_null_enc_id) ==> 
+                (forall m : int :: (m > n && m < kmax_depth_t+1) ==> 
+                    distant_parent(tap_enclave_metadata_owner_map_2, e, m) == tap_null_enc_id)));
 
         // enclave ownermap relationship: Apr 4, 2023.
         //   if the mode_untrusted is from PE's children enclave, then the 2 traces is in **one** children enclave of this PE.
-
-        // invariant ((tap_enclave_metadata_owner_map_1[cpu_enclave_id_1] == eid) ==>
-        //             (cpu_enclave_id_1 == cpu_enclave_id_2));
         invariant ((tap_enclave_metadata_owner_map_1[cpu_enclave_id_1] == eid) ==>
                     (tap_enclave_metadata_valid_2[cpu_enclave_id_2]));
         invariant ((tap_enclave_metadata_owner_map_1[cpu_enclave_id_1] == eid) ==>
@@ -665,9 +683,9 @@ procedure ProveIntegrity()
         // invariants about state sync between 2 traces.
         invariant (current_mode == mode_untrusted) ==> 
             ((tap_enclave_metadata_owner_map_1[cpu_enclave_id_1] != eid) ==> 
-                if is_ancestor(tap_enclave_metadata_owner_map_1, cpu_enclave_id_1, eid)
+                if is_ancestor_EuT(tap_enclave_metadata_owner_map_1, cpu_enclave_id_1, eid)
                     then tap_enclave_metadata_owner_map_2[cpu_enclave_id_2] == eid && 
-                         is_ancestor(tap_enclave_metadata_owner_map_1, cpu_enclave_id_1, cpu_enclave_id_2)
+                         is_ancestor_EuT(tap_enclave_metadata_owner_map_1, cpu_enclave_id_1, cpu_enclave_id_2)
                     else cpu_enclave_id_2 == tap_null_enc_id); 
                     
         invariant (current_mode == mode_untrusted) ==> 
