AbstractPlatform/ProofCommon.bpl
@@ -316,11 +316,24 @@ procedure InitialHavoc(eid: tap_enclave_id_t)
             (tap_enclave_metadata_addr_excl[e][v] <==> cpu_owner_map[tap_enclave_metadata_addr_map[e][v]] == e));
 
     // enclave ownermap relationship: the maximal parent-tree depth is 'n'
+    // maintain 'distant_parent' function
     ensures (forall e : tap_enclave_id_t :: tap_enclave_metadata_valid[e] ==> 
         distant_parent(tap_enclave_metadata_owner_map, e, kmax_depth_t+1) == tap_null_enc_id);
     ensures (forall e : tap_enclave_id_t :: 
         tap_enclave_metadata_valid[e] && tap_enclave_metadata_privileged[e] ==> 
             distant_parent(tap_enclave_metadata_owner_map, e, kmax_depth_t) == tap_null_enc_id);
+    ensures (forall n : int :: 
+        distant_parent(tap_enclave_metadata_owner_map, tap_null_enc_id, n) == tap_null_enc_id);
+    ensures (forall e : tap_enclave_id_t :: tap_enclave_metadata_valid[e] ==> 
+        distant_parent(tap_enclave_metadata_owner_map, e, 1) == tap_enclave_metadata_owner_map[e]);
+    ensures (forall e : tap_enclave_id_t :: tap_enclave_metadata_valid[e] ==> 
+        (forall n1, n2 : int :: (is_valid_depth(n1) && is_valid_depth(n2) && (is_valid_depth(n1 + n2))) ==> 
+            distant_parent(tap_enclave_metadata_owner_map, distant_parent(tap_enclave_metadata_owner_map, e, n1), n2) == 
+            distant_parent(tap_enclave_metadata_owner_map, e, n1 + n2)));
+    ensures (forall e : tap_enclave_id_t :: tap_enclave_metadata_valid[e] ==> 
+        (exists n : int :: (is_valid_depth(n) && (n < kmax_depth_t+1) && distant_parent(tap_enclave_metadata_owner_map, e, n) == tap_null_enc_id) ==> 
+            (forall m : int :: (m > n && m < kmax_depth_t+1) ==> 
+                distant_parent(tap_enclave_metadata_owner_map, e, m) == tap_null_enc_id)));
 
 // launch startup stage.
 procedure LaunchHavoc(eid : tap_enclave_id_t) 
